project/util/NatSet.v
@@ -6,4 +6,3 @@ Definition Node := Nat_as_OT.t.
 
 Module NatSet := FSetList.Make(Nat_as_OT).
 Module NatSetProperties := EqProperties(NatSet).
-
